compose/System.v
@@ -32,7 +32,6 @@ Section SYSMODSEM.
 
   Inductive state: Type :=
   | state_call
-      (fptr_arg: val)
       (rs_arg: regset)
       (m_arg: mem)
   | state_return
@@ -42,8 +41,8 @@ Section SYSMODSEM.
 
   Inductive step (ge: genvtype): state -> trace -> state -> Prop :=
   | step_intro
-      fptr_arg rs_arg m_arg ef
-      (FPTR: ge.(Genv.find_funct) fptr_arg = Some ef)
+      rs_arg m_arg ef
+      (FPTR: ge.(Genv.find_funct) (rs_arg PC) = Some ef)
       vs
       (ARGS: extcall_arguments rs_arg m_arg ef.(ef_sig) vs)
       tr v_ret m_ret
@@ -52,28 +51,28 @@ Section SYSMODSEM.
       (RET: rs_ret = (set_pair (loc_external_result (ef_sig ef)) v_ret
                                (undef_regs (List.map preg_of destroyed_at_call) rs_arg)))
     :
-      step ge (state_call fptr_arg rs_arg m_arg) tr (state_return rs_ret m_ret)
+      step ge (state_call rs_arg m_arg) tr (state_return rs_ret m_ret)
   .
 
   Definition get_mem (st0: state): mem :=
     match st0 with
-    | state_call _ _ m => m
+    | state_call _ m => m
     | state_return _ m => m
     end
   .
 
-  Inductive initial_frame (fptr_arg: val) (rs_arg: regset) (m_arg: mem):
+  Inductive initial_frame (rs_arg: regset) (m_arg: mem):
     state -> Prop :=
   | initial_frame_intro
     :
-      initial_frame fptr_arg rs_arg m_arg (state_call fptr_arg rs_arg m_arg)
+      initial_frame rs_arg m_arg (state_call rs_arg m_arg)
   .
 
-  Inductive final_frame (sg_init: option signature) (rs_init: regset): state -> regset -> mem -> Prop :=
+  Inductive final_frame (rs_init: regset): state -> regset -> mem -> Prop :=
   | final_frame_intro
       rs_ret m_ret
     :
-      final_frame sg_init rs_init (state_return rs_ret m_ret) rs_ret m_ret
+      final_frame rs_init (state_return rs_ret m_ret) rs_ret m_ret
   .
 
   Program Definition modsem: ModSem.t := {|
@@ -81,7 +80,7 @@ Section SYSMODSEM.
     ModSem.genvtype := genvtype;
     ModSem.step := step;
     ModSem.get_mem := get_mem;
-    ModSem.at_external := bot4;
+    ModSem.at_external := bot3;
     ModSem.initial_frame := initial_frame;
     ModSem.final_frame := final_frame;
     ModSem.after_external := bot5;
@@ -89,7 +88,7 @@ Section SYSMODSEM.
   |}
   .
   Next Obligation. inv INIT; ss. Qed.
-  Next Obligation. inv STEP; inv FINAL; ss. Qed.
+  Next Obligation. inv H5; inv H3; ss. Qed.
 
 End SYSMODSEM.
 
